.vscode/Test.v
@@ -1,0 +1,19 @@
+From Ceres Require Import CeresParser.
+From Ceres Require Import Ceres.
+
+From Coq Require Import Ascii.
+From Coq Require Import List.
+Import ListNotations.
+
+From Coq Require Import String.
+Open Scope string_scope.
+
+Definition exp : sexp := Atom_ (Str "hello world ∃ ? .- ၍").
+Definition s : string := string_of_sexp exp.
+Definition exp' := parse_sexp s.
+Definition exp'' := parse_sexp """hello world ∃ ? .- ၍""".
+
+Compute exp.
+Compute s.
+Compute exp'.
+Compute exp''.
